{
 "cells": [
  {
   "cell_type": "markdown",
   "metadata": {},
   "source": [
    "# Name: Rameses Barria\n",
    "# Course: BSCS-1\n",
    "# Id: 23102264\n",
    "# Questions:\n",
    "---\n",
    "\n",
    "1. $\\textbf{Why do we need to prove?}$\n",
    "\n",
    "    We need to prove to establish the validity of a statement or theorem. Proofs provide the logical reasoning that shows that a statement or theorem is correct, allowing us to rely on them for further calculations.\n",
    "    \n",
    "2. $\\textbf{If we fail to generate a proof, what will happen?}$\n",
    "\n",
    "    If we fail to generate a proof, we can't establish the validity of the statement or theorem and use it in further reasoning."
   ]
  },
  {
   "cell_type": "markdown",
   "metadata": {},
   "source": [
    "# 1. Prove that the Euler's number $e = \\Sigma_{k=0}^\\infty \\frac{1}{k!} \\notin \\mathbb{Q}$.\n",
    "---\n",
    "Recall that a rational number is one that can be expressed as the quotient of two integers. We want to prove that Euler's number $e = \\sum_{k=0}^\\infty \\frac{1}{k!} \\notin \\mathbb{Q}$.\n",
    "\n",
    "$\\textit{Proof:}$\n",
    "\n",
    "Assume for contradiction that $e$ is rational, then $e = \\frac{a}{b}$, where $a$ and $b$ are integers and $b \\neq 0$.\n",
    "\n",
    "Consider the series expansion of $e$:\n",
    "\n",
    "\\[ $e = \\sum_{k=0}^\\infty \\frac{1}{k!} = 1 + \\frac{1}{1!} + \\frac{1}{2!} + \\frac{1}{3!} + \\dots $\\]\n",
    "\n",
    "Multiply both sides by $b!$ to clear the denominators:\n",
    "\n",
    "\\[ $b!e = b!\\left(1 + \\frac{1}{1!} + \\frac{1}{2!} + \\frac{1}{3!} + \\dots \\right) = b!(1 + b + \\frac{b(b-1)}{2!} + \\frac{b(b-1)(b-2)}{3!} + \\dots)$ \\]\n",
    "\n",
    "Now, notice that the right side is an integer because every term is a multiple of $b!$. Therefore, $e$ must be rational, contradicting our assumption. Hence, $e \\notin \\mathbb{Q}$."
   ]
  },
  {
   "cell_type": "markdown",
   "metadata": {},
   "source": [
    "# 2. Prove Minkowski's Inequality for sums, $\\forall \\ p>1, (a_k, b_k)>0$:\n",
    "---\n",
    "\n",
    "We want to prove Minkowski's Inequality for sums:\n",
    "\\[ $\\left(\\sum_{k=1}^n |a_k + b_k|^p\\right)^\\frac{1}{p} \\leq \\left(\\sum_{k=1}^n |a_k|^p\\right)^\\frac{1}{p} + \\left(\\sum_{k=1}^n |b_k|^p\\right)^\\frac{1}{p} $\\]\n",
    "\n",
    "$\\textit{Proof:}$\n",
    "\n",
    "The proof involves using Hölder's inequality. Let $q$ be the conjugate exponent of $p$ (i.e., $\\frac{1}{p} + \\frac{1}{q} = 1$).\n",
    "\n",
    "Apply Hölder's inequality with $p$ and $q$ to the sequences $(|a_k|^p)$ and $(1)$, and to the sequences $(|b_k|^p)$ and $(1)$:\n",
    "\n",
    "\\[ $\\sum_{k=1}^n |a_k|^p \\cdot 1 \\leq \\left(\\sum_{k=1}^n |a_k|^p\\right)^\\frac{1}{p} \\left(\\sum_{k=1}^n 1^q\\right)^\\frac{1}{q} = \\left(\\sum_{k=1}^n |a_k|^p\\right)^\\frac{1}{p} \\cdot n^\\frac{1}{q} $\\]\n",
    "\\[ $\\sum_{k=1}^n |b_k|^p \\cdot 1 \\leq \\left(\\sum_{k=1}^n |b_k|^p\\right)^\\frac{1}{p} \\left(\\sum_{k=1}^n 1^q\\right)^\\frac{1}{q} = \\left(\\sum_{k=1}^n |b_k|^p\\right)^\\frac{1}{p} \\cdot n^\\frac{1}{q} $\\]\n",
    "\n",
    "Add these inequalities:\n",
    "\n",
    "\\[ $\\sum_{k=1}^n |a_k|^p + \\sum_{k=1}^n |b_k|^p \\leq \\left(\\sum_{k=1}^n |a_k|^p\\right)^\\frac{1}{p} \\cdot n^\\frac{1}{q} + \\left(\\sum_{k=1}^n |b_k|^p\\right)^\\frac{1}{p} \\cdot n^\\frac{1}{q} $\\]\n",
    "\n",
    "\\[ $\\sum_{k=1}^n (|a_k|^p + |b_k|^p) \\leq \\left(\\sum_{k=1}^n |a_k|^p\\right)^\\frac{1}{p} \\cdot n^\\frac{1}{q} + \\left(\\sum_{k=1}^n |b_k|^p\\right)^\\frac{1}{p} \\cdot n^\\frac{1}{q} $\\]\n",
    "\n",
    "Now, raise both sides to the power of $\\frac{1}{p}$:\n",
    "\n",
    "\\[ $\\left(\\sum_{k=1}^n (|a_k|^p + |b_k|^p)\\right)^\\frac{1}{p} \\leq \\left(\\left(\\sum_{k=1}^n |a_k|^p\\right)^\\frac{1}{p} \\cdot n^\\frac{1}{q} + \\left(\\sum_{k=1}^n |b_k|^p\\right)^\\frac{1}{p} \\cdot n^\\frac{1}{q}\\right)^\\frac{1}{p} $\\]\n",
    "\n",
    "\\[ $\\left(\\sum_{k=1}^n (|a_k + b_k|^p)\\right)^\\frac{1}{p} \\leq \\left(\\sum_{k=1}^n |a_k|^p\\right)^\\frac{1}{p} + \\left(\\sum_{k=1}^n |b_k|^p\\right)^\\frac{1}{p} $\\]\n",
    "\n",
    "Which proves Minkowski's Inequality."
   ]
  },
  {
   "cell_type": "markdown",
   "metadata": {},
   "source": [
    "# 3. Prove the triangle inequality $|x+y| \\leq |x| + |y|, \\forall (x,y) \\in \\mathbb{R}$\n",
    "---\n",
    "\n",
    "$\\textit{Proof:}$\n",
    "\n",
    "Recall the square of a binomial \n",
    "\n",
    "$$\n",
    "(x + y)^{2} = x^{2} + 2xy + y^{2}\n",
    "$$\n",
    "\n",
    "By known property of absolute value, we know that\n",
    "\n",
    "$$\n",
    "x \\leq |x|\\\\\n",
    "y \\leq |y|\\\\\n",
    "$$\n",
    "\n",
    "These inequalities are true for all Real Numbers\n",
    "\n",
    "$$\n",
    "x^{2} + 2xy + y^{2} \\leq |x|^{2} + 2|x||y| + |x|^{2}\n",
    "$$\n",
    "\n",
    "$$\n",
    "(x+y)^{2} \\leq |x|^{2} + 2|x||y| + |y|^{2}\n",
    "$$\n",
    "\n",
    "factor out $2|x||y|$\n",
    "\n",
    "$$\n",
    "(x+y)^{2} \\leq |x|^{2} + |y|^{2}\n",
    "$$\n",
    "\n",
    "By known property of absolute values, we know that\n",
    "\n",
    "$$\n",
    "\\forall x \\in \\mathbb{R}\\\\\n",
    "\n",
    "\\sqrt{x^{2}} = |x|\\\\\n",
    "$$\n",
    "\n",
    "Therefore if we square root all terms,\n",
    "\n",
    "$$\n",
    "\\sqrt{(x+y)^{2}} \\leq \\sqrt{|x|^{2}} + \\sqrt{|y|^{2}}\n",
    "$$\n",
    "\n",
    "Is equivalent to\n",
    "\n",
    "$$\n",
    "|x + y| \\leq |x| + |y|\n",
    "$$"
   ]
  },
  {
   "cell_type": "markdown",
   "metadata": {},
   "source": [
    "# 4. Prove Sedrakayan's Lemma $\\forall u_i, v_i \\in \\mathbb{R}^+$:\n",
    "---\n",
    "\n",
    "Prove Sedrakayan's Lemma $\\forall u_i, v_i \\in \\mathbb{R}^+$:\n",
    "\n",
    "$\\frac{(\\sum_{i=1}^n u_i)^2}{\\sum_{i=1}^n v_i} \\leq \\sum_{i=1}^n \\frac{(u_i)^2}{v_i}$\n",
    "\n",
    "$\\textit{Proof:}$\n",
    "\n",
    "Let $\\mathbf{u} = (u_1, u_2, ..., u_n)$ and $\\mathbf{v} = (v_1, v_2, ..., v_n)$ be vectors in $\\mathbb{R}^+$.\n",
    "\n",
    "By Cauchy-Schwarz Inequality...\n",
    "\n",
    "For the sum of $u_i$, we have:\n",
    "- $\\left(\\sum_{i=1}^n u_i\\right)^2 \\leq n \\left(\\sum_{i=1}^n u_i^2\\right)$\n",
    "\n",
    "For the sum of $\\sqrt{v_i}$, we have:\n",
    "- $\\left(\\sum_{i=1}^n \\sqrt{v_i}\\right)^2 \\leq n \\left(\\sum_{i=1}^n v_i\\right)$\n",
    "\n",
    "Rearrange the Equation:\n",
    "\n",
    "Rearranging, we get:\n",
    "- $\\frac{\\left(\\sum_{i=1}^n u_i\\right)^2}{\\sum_{i=1}^n v_i} \\leq \\frac{\\sum_{i=1}^n u_i^2}{\\sum_{i=1}^n v_i}$\n",
    "\n",
    "<b>Step 5: </b> Acknowledge the obtained expression as the final form:\n",
    "\\begin{gathered} \\frac{\\left(\\sum_{i=1}^n u_i\\right)^2}{\\sum_{i=1}^n v_i} \\leq \\frac{\\sum_{i=1}^n u_i^2}{\\sum_{i=1}^n v_i} \\end{gathered}"
   ]
  },
  {
   "cell_type": "markdown",
   "metadata": {},
   "source": [
    "### $\\textbf{Extra Problems}$\n",
    "\n",
    "1. Consider the functions $f(x) = 2x+1$, $g(x)=2y-1$, $j(x) = |f(x)+g(x)|$, and $h(x) = j(x)^2$, show for the following inequality that:\n",
    "\\begin{gathered}\n",
    "\\sqrt{|f(x)|^2} \\geq \\sqrt{h(x)} - \\sqrt{|g(x)|^2}, \\forall (x,y) \\in \\mathbb{Z}^+\n",
    "\\end{gathered}\n",
    "\n",
    "---\n",
    "\n",
    "$\\textbf{Answer:}$\n",
    "\n",
    "Substitution\n",
    "\n",
    "\\begin{gathered}\n",
    "\\sqrt{\\left|f\\left(x\\right)\\right|^2}\\ge \\sqrt{\\left|f\\left(x\\right)+g\\left(x\\right)\\right|^2}-\\sqrt{\\left|g\\left(x\\right)\\right|^2}\n",
    "\\end{gathered}\n",
    "\n",
    "Minkowski's Inequality for sums\n",
    "\n",
    "\\begin{gathered}\n",
    "\\left|f\\left(x\\right)\\right|\\ge \\left|f\\left(x\\right)+g\\left(x\\right)\\right|-\\left|g\\left(x\\right)\\right|\n",
    "\\end{gathered}\n",
    "\n",
    "Transpose\n",
    "\n",
    "\\begin{gathered}\n",
    "\\left|f\\left(x\\right)\\right|+\\left|g\\left(x\\right)\\right|\\ge \\left|f\\left(x\\right)+g\\left(x\\right)\\right|\n",
    "\\end{gathered}\n",
    "\n",
    "Rearrange to Triangle Inequality\n",
    "\n",
    "\\begin{gathered}\n",
    "\\left|f\\left(x\\right)+g\\left(x\\right)\\right|\\le \\left|f\\left(x\\right)\\right|+\\left|g\\left(x\\right)\\right|\n",
    "\\end{gathered}\n",
    "\n",
    "Prove with the case: $f\\left(x\\right)>0$, and $g\\left(x\\right)>0$, Since $\\forall (x,y) \\in \\mathbb{Z}^+$\n",
    "\n",
    "- Let $\\left|f\\left(x\\right)+g\\left(x\\right)\\right|=f\\left(x\\right)+g\\left(x\\right)$, and $|x|=x$, $|y|=y$\n",
    "\n",
    "- Substitute:\n",
    "\\begin{gathered}\n",
    "\\left|f\\left(x\\right)+g\\left(x\\right)\\right|=f\\left(x\\right)+g\\left(x\\right)=\\left|f\\left(x\\right)\\right|+\\left|g\\left(x\\right)\\right|\n",
    "\\end{gathered}\n",
    "\n",
    "<br><br>"
   ]
  },
  {
   "cell_type": "markdown",
   "metadata": {},
   "source": [
    "2. Prove Sedrakayan's Lemma if $u_i, v_i$ are square roots of an even integers:\n",
    "\\begin{gathered}\n",
    "\\frac{(\\Sigma_{i=1}^n u_i)^2}{\\Sigma_{i=1}^n v_i}\n",
    "\\leq\n",
    "\\Sigma_{i=1}^n \\frac{(u_i)^2}{v_i}\n",
    "\\end{gathered}\n",
    "---\n",
    "$\\textbf{Answer:}$\n",
    "\n",
    "To prove Sedrakayan's Lemma when $ u_i $ and $ v_i $ are square roots of even integers:\n",
    "\n",
    "Let $ u_i = \\sqrt{2a_i} $ and $ v_i = \\sqrt{2b_i} $, where $ a_i $ and $ b_i $ are positive integers. We need to show:\n",
    "\n",
    "$$\n",
    "\\frac{\\left( \\sum_{i=1}^n \\sqrt{2a_i} \\right)^2}{\\sum_{i=1}^n \\sqrt{2b_i}} \\leq \\sum_{i=1}^n \\frac{(2a_i)}{(2b_i)}\n",
    "$$\n",
    "\n",
    "Expand the terms\n",
    "\n",
    "- Expanding the terms, we get:\n",
    "$$\n",
    "\\frac{\\left( \\sum_{i=1}^n \\sqrt{2a_i} \\right)^2}{\\sum_{i=1}^n \\sqrt{2b_i}} = \\frac{\\left( \\sum_{i=1}^n \\sqrt{2a_i} \\right) \\left( \\sum_{i=1}^n \\sqrt{2a_i} \\right)}{\\sum_{i=1}^n \\sqrt{2b_i}}\n",
    ", \\quad\n",
    "\\sum_{i=1}^n \\frac{(2a_i)}{(2b_i)} = \\sum_{i=1}^n \\frac{2a_i}{2b_i}\n",
    "$$\n",
    "\n",
    "\n",
    "Rewrite\n",
    "\n",
    "- Since $ \\sqrt{2a_i} $ and $ \\sqrt{2b_i} $ are positive, we can rewrite the inequality as:\n",
    "$$\n",
    "\\frac{\\left( \\sum_{i=1}^n \\sqrt{2a_i} \\right)^2}{\\sum_{i=1}^n \\sqrt{2b_i}} \\leq \\sum_{i=1}^n \\frac{\\sqrt{2a_i}^2}{\\sqrt{2b_i}}\n",
    "$$\n",
    "\n",
    "Consider the identity:\n",
    "\n",
    "- Now, consider the following identity:\n",
    "$$\n",
    "\\left( \\sum_{i=1}^n x_i \\right)^2 = \\sum_{i=1}^n x_i^2 + 2 \\sum_{1 \\leq i < j \\leq n} x_i x_j\n",
    "$$\n",
    "\n",
    "Apply the identity\n",
    "\n",
    "- Applying this identity to the numerator, we get:\n",
    "$$\n",
    "\\frac{\\left( \\sum_{i=1}^n \\sqrt{2a_i} \\right)^2}{\\sum_{i=1}^n \\sqrt{2b_i}} = \\frac{\\sum_{i=1}^n (2a_i) + 2 \\sum_{1 \\leq i < j \\leq n} \\sqrt{2a_i} \\sqrt{2a_j}}{\\sum_{i=1}^n \\sqrt{2b_i}}\n",
    "$$\n",
    "\n",
    "Consider the following:\n",
    "\n",
    "- Since $2a_i$ and $2b_i$ are even integers, $2 \\sum_{1 \\leq i < j \\leq n} \\sqrt{2a_i} \\sqrt{2a_j}$ is also even.\n",
    "- Now, we have:\n",
    "$$\n",
    "\\frac{\\sum_{i=1}^n (2a_i)}{\\sum_{i=1}^n \\sqrt{2b_i}} + \\frac{2 \\sum_{1 \\leq i < j \\leq n} \\sqrt{2a_i} \\sqrt{2a_j}}{\\sum_{i=1}^n \\sqrt{2b_i}} \\leq \\sum_{i=1}^n \\frac{(2a_i)}{\\sqrt{2b_i}}\n",
    "$$\n",
    "\n",
    "Simplify the expression\n",
    "$$\n",
    "\\frac{\\sum_{i=1}^n (2a_i)}{\\sum_{i=1}^n \\sqrt{2b_i}} \\leq \\sum_{i=1}^n \\frac{(2a_i)}{\\sqrt{2b_i}}\n",
    "$$\n",
    "\n",
    "Given that both sides of the inequality consist of non-negative terms, and the numerator on the left-hand side includes the terms from the denominator on the right-hand side, the inequality is valid. Thus, Sedrakayan's Lemma is confirmed for $ u_i $ and $ v_i $ as square roots of even integers.\n",
    "\n",
    "\n",
    "\n"
   ]
  }
 ],
 "metadata": {
  "language_info": {
   "name": "python"
  }
 },
 "nbformat": 4,
 "nbformat_minor": 2
}
